src/model/Local.v
@@ -1,0 +1,759 @@
+Require Import RelationClasses.
+
+From sflib Require Import sflib.
+
+From PromisingLib Require Import Axioms.
+From PromisingLib Require Import Basic.
+From PromisingLib Require Import DataStructure.
+From PromisingLib Require Import DenseOrder.
+From PromisingLib Require Import Loc.
+From PromisingLib Require Import Event.
+
+Require Import Time.
+Require Import View.
+Require Import Promises.
+Require Import Reserves.
+Require Import Cell.
+Require Import Memory.
+Require Import TView.
+Require Import Global.
+
+Set Implicit Arguments.
+
+
+Module ThreadEvent.
+  Variant t :=
+  | promise (loc: Loc.t)
+  | reserve (loc: Loc.t) (ts: Time.t)
+  | cancel (loc: Loc.t) (ts: Time.t)
+  | silent
+  | read (loc: Loc.t) (ts: Time.t) (val: Const.t) (released: option View.t) (ord: Ordering.t)
+  | write (loc: Loc.t) (from to: Time.t) (val: Const.t) (released: option View.t) (ord: Ordering.t)
+  | update (loc: Loc.t) (tsr tsw: Time.t) (valr valw: Const.t)
+           (releasedr releasedw: option View.t) (ordr ordw: Ordering.t)
+  | fence (ordr ordw: Ordering.t)
+  | syscall (e: Event.t)
+  | failure
+  | racy_read (loc: Loc.t) (to: option Time.t) (val: Const.t) (ord: Ordering.t)
+  | racy_write (loc: Loc.t) (to: option Time.t) (val: Const.t) (ord: Ordering.t)
+  | racy_update (loc: Loc.t) (to: option Time.t) (valr valw: Const.t) (ordr ordw: Ordering.t)
+  .
+  #[global] Hint Constructors t: core.
+
+  Definition get_event (e: t): option Event.t :=
+    match e with
+    | syscall e => Some e
+    | _ => None
+    end.
+
+  Definition get_program_event (e: t): ProgramEvent.t :=
+    match e with
+    | promise _
+    | reserve _ _
+    | cancel _ _
+    | silent => ProgramEvent.silent
+    | read loc _ val _ ord => ProgramEvent.read loc val ord
+    | write loc _ _ val _ ord => ProgramEvent.write loc val ord
+    | update loc _ _ valr valw _ _ ordr ordw => ProgramEvent.update loc valr valw ordr ordw
+    | fence ordr ordw => ProgramEvent.fence ordr ordw
+    | syscall ev => ProgramEvent.syscall ev
+    | failure => ProgramEvent.failure
+    | racy_read loc _ val ord => ProgramEvent.read loc val ord
+    | racy_write loc _ val ord => ProgramEvent.write loc val ord
+    | racy_update loc _ valr valw ordr ordw => ProgramEvent.update loc valr valw ordr ordw
+    end.
+
+  Definition get_machine_event (e: t): MachineEvent.t :=
+    match e with
+    | syscall e => MachineEvent.syscall e
+    | failure
+    | racy_write _ _ _ _
+    | racy_update _ _ _ _ _ _ => MachineEvent.failure
+    | _ => MachineEvent.silent
+    end.
+
+  Definition get_machine_event_pf (e: t): MachineEvent.t :=
+    match e with
+    | syscall e => MachineEvent.syscall e
+    | failure
+    | racy_read _ _ _ _
+    | racy_write _ _ _ _
+    | racy_update _ _ _ _ _ _ => MachineEvent.failure
+    | _ => MachineEvent.silent
+    end.
+
+  Definition is_reading (e:t): option (Loc.t * Time.t * Const.t * option View.t * Ordering.t) :=
+    match e with
+    | read loc ts val released ord => Some (loc, ts, val, released, ord)
+    | update loc tsr _ valr _ releasedr _ ordr _ => Some (loc, tsr, valr, releasedr, ordr)
+    | _ => None
+    end.
+
+  Definition is_writing (e:t): option (Loc.t * Time.t * Time.t * Const.t * option View.t * Ordering.t) :=
+    match e with
+    | write loc from to val released ord => Some (loc, from, to, val, released, ord)
+    | update loc tsr tsw _ valw _ releasedw _ ordw => Some (loc, tsr, tsw, valw, releasedw, ordw)
+    | _ => None
+    end.
+
+  Definition is_accessing (e:t): option (Loc.t * Time.t) :=
+    match e with
+    | read loc ts _ _ _ => Some (loc, ts)
+    | write loc _ ts _ _ _ => Some (loc, ts)
+    | update loc _ ts _ _ _ _ _ _ => Some (loc, ts)
+    | _ => None
+    end.
+
+  Definition is_accessing_loc (l: Loc.t) (e: t): Prop :=
+    match e with
+    | read loc _ _ _ _
+    | write loc _ _ _ _ _
+    | update loc _ _ _ _ _ _ _ _
+    | racy_read loc _ _ _
+    | racy_write loc _ _ _
+    | racy_update loc _ _ _ _ _ => loc = l
+    | _ => False
+    end.
+
+  Lemma eq_program_event_eq_loc
+        e1 e2 loc
+        (EVENT: get_program_event e1 = get_program_event e2):
+    is_accessing_loc loc e1 <-> is_accessing_loc loc e2.
+  Proof.
+    unfold is_accessing_loc.
+    destruct e1, e2; ss; inv EVENT; ss.
+  Qed.
+End ThreadEvent.
+
+
+Module Local.
+  Structure t := mk {
+    tview: TView.t;
+    promises: Promises.t;
+    reserves: Reserves.t;
+  }.
+
+  Definition init := mk TView.bot Promises.bot Reserves.bot.
+
+  Variant is_terminal (lc:t): Prop :=
+  | is_terminal_intro
+      (PROMISES: promises lc = Promises.bot)
+  .
+  #[global] Hint Constructors is_terminal: core.
+
+  Variant wf (lc: t) (gl: Global.t): Prop :=
+  | wf_intro
+      (TVIEW_WF: TView.wf (tview lc))
+      (TVIEW_CLOSED: TView.closed (tview lc) (Global.memory gl))
+      (PROMISES: Promises.le (promises lc) (Global.promises gl))
+      (PROMISES_FINITE: Promises.finite (promises lc))
+      (RESERVES: Reserves.incl (reserves lc) (Global.reserves gl))
+      (RESERVES_FINITE: Reserves.finite (reserves lc))
+      (RESERVES_CLOSED: Memory.closed_reserves (reserves lc) (Global.memory gl))
+  .
+  #[global] Hint Constructors wf: core.
+
+  Variant disjoint (lc1 lc2:t): Prop :=
+  | disjoint_intro
+      (PROMISES_DISJOINT: Promises.disjoint (promises lc1) (promises lc2))
+      (RESERVES_DISJOINT: Reserves.disjoint (reserves lc1) (reserves lc2))
+  .
+  #[global] Hint Constructors disjoint: core.
+
+  Global Program Instance disjoint_Symmetric: Symmetric disjoint.
+  Next Obligation.
+    econs; symmetry; apply H.
+  Qed.
+
+
+  Variant promise_step (lc1: t) (gl1: Global.t) (loc: Loc.t) (lc2: t) (gl2: Global.t): Prop :=
+  | promise_step_intro
+      prm2 gprm2
+      (PROMISE: Promises.promise (promises lc1) (Global.promises gl1) loc prm2 gprm2)
+      (LC2: lc2 = mk (tview lc1) prm2 (reserves lc1))
+      (GL2: gl2 = Global.mk (Global.sc gl1) gprm2 (Global.reserves gl1) (Global.memory gl1))
+  .
+  #[global] Hint Constructors promise_step: core.
+
+  Variant reserve_step (lc1: t) (gl1: Global.t) (loc: Loc.t) (ts: Time.t) (lc2: t) (gl2: Global.t): Prop :=
+  | reserve_step_intro
+      from msg
+      rsv2 grsv2
+      (TS: Memory.get loc ts (Global.memory gl1) = Some (from, msg))
+      (RESERVE: Reserves.reserve (reserves lc1) (Global.reserves gl1) loc ts rsv2 grsv2)
+      (LC2: lc2 = mk (tview lc1) (promises lc1) rsv2)
+      (GL2: gl2 = Global.mk (Global.sc gl1) (Global.promises gl1) grsv2 (Global.memory gl1))
+  .
+  #[global] Hint Constructors reserve_step: core.
+
+  Variant cancel_step (lc1: t) (gl1: Global.t) (loc: Loc.t) (ts: Time.t) (lc2: t) (gl2: Global.t): Prop :=
+  | cancel_step_intro
+      rsv2 grsv2
+      (CANCEL: Reserves.cancel (reserves lc1) (Global.reserves gl1) loc ts rsv2 grsv2)
+      (LC2: lc2 = mk (tview lc1) (promises lc1) rsv2)
+      (GL2: gl2 = Global.mk (Global.sc gl1) (Global.promises gl1) grsv2 (Global.memory gl1))
+  .
+  #[global] Hint Constructors cancel_step: core.
+
+  Variant read_step
+          (lc1: t) (gl1: Global.t)
+          (loc: Loc.t) (to: Time.t) (val: Const.t) (released: option View.t) (ord: Ordering.t)
+          (lc2: t): Prop :=
+  | read_step_intro
+      from val' na
+      tview2
+      (GET: Memory.get loc to (Global.memory gl1) = Some (from, Message.mk val' released na))
+      (VAL: Const.le val val')
+      (READABLE: TView.readable (TView.cur (tview lc1)) loc to released ord)
+      (TVIEW: TView.read_tview (tview lc1) loc to released ord = tview2)
+      (LC2: lc2 = mk tview2 (promises lc1) (reserves lc1)):
+      read_step lc1 gl1 loc to val released ord lc2
+  .
+  #[global] Hint Constructors read_step: core.
+
+  Variant write_step
+          (lc1: t) (gl1: Global.t)
+          (loc: Loc.t) (from to: Time.t)
+          (val: Const.t) (releasedm released: option View.t) (ord: Ordering.t)
+          (lc2: t) (gl2: Global.t): Prop :=
+  | write_step_intro
+      mem2
+      (RELEASED: released = TView.write_released (tview lc1) (Global.sc gl1) loc to releasedm ord)
+      (WRITABLE: TView.writable (TView.cur (tview lc1)) (Global.sc gl1) loc to ord)
+      (NON_RESERVED: forall ts (GET: (Global.reserves gl1) loc = Some ts), Time.lt ts from)
+      (WRITE: Memory.add (Global.memory gl1) loc from to
+                         (Message.mk val released (Ordering.le ord Ordering.na)) mem2)
+      (LC2: lc2 = mk (TView.write_tview (tview lc1) (Global.sc gl1) loc to ord) (promises lc1) (reserves lc1))
+      (GL2: gl2 = Global.mk (Global.sc gl1) (Global.promises gl1) (Global.reserves gl1) mem2):
+      write_step lc1 gl1 loc from to val releasedm released ord lc2 gl2
+  .
+  #[global] Hint Constructors write_step: core.
+
+  Variant fence_step (lc1: t) (gl1: Global.t) (ordr ordw: Ordering.t) (lc2: t) (gl2: Global.t): Prop :=
+  | fence_step_intro
+      tview2
+      (READ: TView.read_fence_tview (tview lc1) ordr = tview2)
+      (LC2: lc2 = mk (TView.write_fence_tview tview2 (Global.sc gl1) ordw)
+                     (promises lc1) (reserves lc1))
+      (GL2: gl2 = Global.mk (TView.write_fence_sc tview2 (Global.sc gl1) ordw)
+                            (Global.promises gl1) (Global.reserves gl1) (Global.memory gl1))
+      (PROMISES: ordw = Ordering.seqcst -> promises lc1 = Promises.bot):
+      fence_step lc1 gl1 ordr ordw lc2 gl2
+  .
+  #[global] Hint Constructors fence_step: core.
+
+  Variant failure_step (lc1:t): Prop :=
+  | failure_step_intro
+  .
+  #[global] Hint Constructors failure_step: core.
+
+  Variant is_racy (lc1: t) (gl1: Global.t) (loc: Loc.t): forall (to: option Time.t) (ord: Ordering.t), Prop :=
+  | is_racy_promise
+      ord
+      (GET: (Global.promises gl1) loc = true)
+      (GETP: (promises lc1) loc = false):
+    is_racy lc1 gl1 loc None ord
+  | is_racy_message
+      to from val released na ord
+      (GET: Memory.get loc to (Global.memory gl1) = Some (from, Message.mk val released na))
+      (RACE: TView.racy_view (TView.cur (tview lc1)) loc to)
+      (MSG: Ordering.le Ordering.plain ord -> na = true):
+    is_racy lc1 gl1 loc (Some to) ord
+  .
+  #[global] Hint Constructors is_racy: core.
+
+  Variant racy_read_step (lc1: t) (gl1: Global.t) (loc: Loc.t) (to: option Time.t) (val:Const.t) (ord:Ordering.t): Prop :=
+  | racy_read_step_intro
+      (RACE: is_racy lc1 gl1 loc to ord)
+  .
+  #[global] Hint Constructors racy_read_step: core.
+
+  Variant racy_write_step (lc1: t) (gl1: Global.t) (loc: Loc.t) (to: option Time.t) (ord: Ordering.t): Prop :=
+  | racy_write_step_intro
+      (RACE: is_racy lc1 gl1 loc to ord)
+  .
+  #[global] Hint Constructors racy_write_step: core.
+
+  Variant racy_update_step (lc1: t) (gl1: Global.t) (loc: Loc.t):
+    forall (to: option Time.t) (ordr ordw: Ordering.t), Prop :=
+  | racy_update_step_ordr
+      ordr ordw
+      (ORDR: Ordering.le ordr Ordering.na):
+    racy_update_step lc1 gl1 loc None ordr ordw
+  | racy_update_step_ordw
+      ordr ordw
+      (ORDW: Ordering.le ordw Ordering.na):
+    racy_update_step lc1 gl1 loc None ordr ordw
+  | racy_update_step_race
+      to ordr ordw
+      (RACE: is_racy lc1 gl1 loc to ordr):
+    racy_update_step lc1 gl1 loc to ordr ordw
+  .
+  #[global] Hint Constructors racy_update_step: core.
+
+
+  Variant internal_step:
+    forall (e: ThreadEvent.t) (lc1: t) (gl1: Global.t) (lc2: t) (gl2: Global.t), Prop :=
+  | step_promise
+      lc1 gl1 
+      loc lc2 gl2
+      (LOCAL: promise_step lc1 gl1 loc lc2 gl2):
+    internal_step (ThreadEvent.promise loc) lc1 gl1 lc2 gl2
+  | step_reserve
+      lc1 gl1 
+      loc ts lc2 gl2
+      (LOCAL: reserve_step lc1 gl1 loc ts lc2 gl2):
+    internal_step (ThreadEvent.reserve loc ts) lc1 gl1 lc2 gl2
+  | step_cancel
+      lc1 gl1 
+      loc ts lc2 gl2
+      (LOCAL: cancel_step lc1 gl1 loc ts lc2 gl2):
+    internal_step (ThreadEvent.cancel loc ts) lc1 gl1 lc2 gl2
+  .
+
+  Variant program_step:
+    forall (e: ThreadEvent.t) (lc1: t) (gl1: Global.t) (lc2: t) (gl2: Global.t), Prop :=
+  | step_silent
+      lc1 gl1:
+    program_step ThreadEvent.silent lc1 gl1 lc1 gl1
+  | step_read
+      lc1 gl1
+      loc to val released ord lc2
+      (LOCAL: read_step lc1 gl1 loc to val released ord lc2):
+    program_step (ThreadEvent.read loc to val released ord) lc1 gl1 lc2 gl1
+  | step_write
+      lc1 gl1
+      loc from to val released ord lc2 gl2
+      (LOCAL: write_step lc1 gl1 loc from to val None released ord lc2 gl2):
+    program_step (ThreadEvent.write loc from to val released ord) lc1 gl1 lc2 gl2
+  | step_update
+      lc1 gl1
+      loc ordr ordw
+      tsr valr releasedr releasedw lc2
+      tsw valw lc3 gl3
+      (LOCAL1: read_step lc1 gl1 loc tsr valr releasedr ordr lc2)
+      (LOCAL2: write_step lc2 gl1 loc tsr tsw valw releasedr releasedw ordw lc3 gl3):
+    program_step (ThreadEvent.update loc tsr tsw valr valw releasedr releasedw ordr ordw)
+                 lc1 gl1 lc3 gl3
+  | step_fence
+      lc1 gl1
+      ordr ordw lc2 gl2
+      (LOCAL: fence_step lc1 gl1 ordr ordw lc2 gl2):
+    program_step (ThreadEvent.fence ordr ordw) lc1 gl1 lc2 gl2
+  | step_syscall
+      lc1 gl1
+      e lc2 gl2
+      (LOCAL: fence_step lc1 gl1 Ordering.seqcst Ordering.seqcst lc2 gl2):
+    program_step (ThreadEvent.syscall e) lc1 gl1 lc2 gl2
+  | step_failure
+      lc1 gl1
+      (LOCAL: failure_step lc1):
+    program_step ThreadEvent.failure lc1 gl1 lc1 gl1
+  | step_racy_read
+      lc1 gl1
+      loc to val ord
+      (LOCAL: racy_read_step lc1 gl1 loc to val ord):
+    program_step (ThreadEvent.racy_read loc to val ord) lc1 gl1 lc1 gl1
+  | step_racy_write
+      lc1 gl1
+      loc to val ord
+      (LOCAL: racy_write_step lc1 gl1 loc to ord):
+    program_step (ThreadEvent.racy_write loc to val ord) lc1 gl1 lc1 gl1
+  | step_racy_update
+      lc1 gl1
+      loc to valr valw ordr ordw
+      (LOCAL: racy_update_step lc1 gl1 loc to ordr ordw):
+    program_step (ThreadEvent.racy_update loc to valr valw ordr ordw) lc1 gl1 lc1 gl1
+  .
+  #[global] Hint Constructors program_step: core.
+
+
+  (* step_future *)
+
+  Lemma promise_step_future
+        lc1 gl1 loc lc2 gl2
+        (STEP: promise_step lc1 gl1 loc lc2 gl2)
+        (LC_WF1: wf lc1 gl1)
+        (GL_WF1: Global.wf gl1):
+    <<LC_WF2: wf lc2 gl2>> /\
+    <<GL_WF2: Global.wf gl2>> /\
+    <<SC_FUTURE: TimeMap.le (Global.sc gl1) (Global.sc gl2)>> /\
+    <<MEM_FUTURE: Memory.future (Global.memory gl1) (Global.memory gl2)>>.
+  Proof.
+    inv LC_WF1. inv GL_WF1. inv STEP. ss.
+    hexploit Promises.promise_le; eauto. i.
+    hexploit Promises.promise_finite; eauto. i.
+    splits; ss; refl.
+  Qed.
+
+  Lemma add_closed_reserves
+        rsv1 loc ts rsv2 mem from msg
+        (GET: Memory.get loc ts mem = Some (from, msg))
+        (ADD: Reserves.add rsv1 loc ts rsv2)
+        (CLOSED: Memory.closed_reserves rsv1 mem):
+    Memory.closed_reserves rsv2 mem.
+  Proof.
+    ii. revert GET0. inv ADD.
+    unfold LocFun.add. condtac; ss; eauto. i. clarify.
+    destruct msg. esplits; eauto.
+  Qed.
+
+  Lemma reserve_step_future
+        lc1 gl1 loc ts lc2 gl2
+        (STEP: reserve_step lc1 gl1 loc ts lc2 gl2)
+        (LC_WF1: wf lc1 gl1)
+        (GL_WF1: Global.wf gl1):
+    <<LC_WF2: wf lc2 gl2>> /\
+    <<GL_WF2: Global.wf gl2>> /\
+    <<TVIEW_FUTURE: TView.le (tview lc1) (tview lc2)>> /\
+    <<SC_FUTURE: TimeMap.le (Global.sc gl1) (Global.sc gl2)>> /\
+    <<MEM_FUTURE: Memory.future (Global.memory gl1) (Global.memory gl2)>>.
+  Proof.
+    inv LC_WF1. inv GL_WF1. inv STEP. ss.
+    hexploit Reserves.reserve_incl; eauto. i.
+    hexploit Reserves.reserve_finite; eauto. i.
+    inv RESERVE.
+    splits; try refl; econs; ss;
+      eauto using add_closed_reserves.
+  Qed.
+
+  Lemma remove_closed_reserves
+        rsv1 loc ts rsv2 mem
+        (REMOVE: Reserves.remove rsv1 loc ts rsv2)
+        (CLOSED: Memory.closed_reserves rsv1 mem):
+    Memory.closed_reserves rsv2 mem.
+  Proof.
+    ii. revert GET. inv REMOVE.
+    unfold LocFun.add. condtac; ss; eauto.
+  Qed.
+
+  Lemma cancel_step_future
+        lc1 gl1 loc ts lc2 gl2
+        (STEP: cancel_step lc1 gl1 loc ts lc2 gl2)
+        (LC_WF1: wf lc1 gl1)
+        (GL_WF1: Global.wf gl1):
+    <<LC_WF2: wf lc2 gl2>> /\
+    <<GL_WF2: Global.wf gl2>> /\
+    <<TVIEW_FUTURE: TView.le (tview lc1) (tview lc2)>> /\
+    <<SC_FUTURE: TimeMap.le (Global.sc gl1) (Global.sc gl2)>> /\
+    <<MEM_FUTURE: Memory.future (Global.memory gl1) (Global.memory gl2)>>.
+  Proof.
+    inv LC_WF1. inv GL_WF1. inv STEP. ss.
+    hexploit Reserves.cancel_incl; eauto. i.
+    hexploit Reserves.cancel_finite; eauto. i.
+    inv CANCEL.
+    splits; try refl; econs; ss;
+      eapply remove_closed_reserves; eauto.
+  Qed.
+
+  Lemma read_step_future
+        lc1 gl1 loc ts val released ord lc2
+        (STEP: read_step lc1 gl1 loc ts val released ord lc2)
+        (LC_WF1: wf lc1 gl1)
+        (GL_WF1: Global.wf gl1):
+    <<LC_WF2: wf lc2 gl1>> /\
+    <<TVIEW_FUTURE: TView.le (tview lc1) (tview lc2)>> /\
+    <<REL_WF: View.opt_wf released>> /\
+    <<REL_CLOSED: Memory.closed_opt_view released (Global.memory gl1)>> /\
+    <<REL_TS: Time.le (View.rlx (View.unwrap released) loc) ts>>.
+  Proof.
+    inv LC_WF1. inv GL_WF1. inv STEP. ss.
+    dup MEM_CLOSED. inv MEM_CLOSED0. exploit CLOSED; eauto. i. des.
+    inv MSG_WF. inv MSG_CLOSED. inv MSG_TS.
+    exploit TViewFacts.read_future; try exact GET; eauto.
+    i. des. splits; auto.
+    - econs; eauto.
+    - apply TViewFacts.read_tview_incr.
+  Qed.
+
+  Lemma write_step_future
+        lc1 gl1 loc from to val releasedm released ord lc2 gl2
+        (STEP: write_step lc1 gl1 loc from to val releasedm released ord lc2 gl2)
+        (REL_WF: View.opt_wf releasedm)
+        (REL_CLOSED: Memory.closed_opt_view releasedm (Global.memory gl1))
+        (REL_TS: Time.le (View.rlx (View.unwrap releasedm) loc) to)
+        (LC_WF1: wf lc1 gl1)
+        (GL_WF1: Global.wf gl1):
+    <<LC_WF2: wf lc2 gl2>> /\
+    <<GL_WF2: Global.wf gl2>> /\
+    <<TVIEW_FUTURE: TView.le (tview lc1) (tview lc2)>> /\
+    <<SC_FUTURE: TimeMap.le (Global.sc gl1) (Global.sc gl2)>> /\
+    <<MEM_FUTURE: Memory.future (Global.memory gl1) (Global.memory gl2)>> /\
+    <<REL_WF: View.opt_wf released>> /\
+    <<REL_TS: Time.le ((View.rlx (View.unwrap released)) loc) to>> /\
+    <<REL_CLOSED: Memory.closed_opt_view released (Global.memory gl2)>>.
+  Proof.
+    inv LC_WF1. inv GL_WF1. inv STEP. ss.
+    exploit TViewFacts.write_future; eauto. s. i. des.
+    exploit Memory.add_future; try apply WRITE; eauto.
+    { econs. eapply TViewFacts.write_released_ts; eauto. }
+    i. des.
+    exploit Memory.add_get0; try apply WRITE; eauto. i. des.
+    splits; eauto.
+    - econs; eauto. s.
+      eapply Memory.add_closed_reserves; eauto.
+    - econs; eauto. s.
+      eapply Memory.add_closed_reserves; eauto.
+    - apply TViewFacts.write_tview_incr. auto.
+    - refl.
+    - eapply TViewFacts.write_released_ts; eauto.
+  Qed.
+
+  Lemma fence_step_future
+        lc1 gl1 ordr ordw lc2 gl2
+        (STEP: fence_step lc1 gl1 ordr ordw lc2 gl2)
+        (LC_WF1: wf lc1 gl1)
+        (GL_WF1: Global.wf gl1):
+    <<LC_WF2: wf lc2 gl2>> /\
+    <<GL_WF2: Global.wf gl2>> /\
+    <<TVIEW_FUTURE: TView.le (tview lc1) (tview lc2)>> /\
+    <<SC_FUTURE: TimeMap.le (Global.sc gl1) (Global.sc gl2)>> /\
+    <<MEM_FUTURE: Memory.future (Global.memory gl1) (Global.memory gl2)>>.
+  Proof.
+    inv LC_WF1. inv GL_WF1. inv STEP. ss.
+    exploit TViewFacts.read_fence_future; eauto. i. des.
+    exploit TViewFacts.write_fence_future; eauto. i. des.
+    splits; eauto.
+    - econs; ss.
+    - etrans.
+      + apply TViewFacts.write_fence_tview_incr. auto.
+      + apply TViewFacts.write_fence_tview_mon; eauto; try refl.
+        apply TViewFacts.read_fence_tview_incr. auto.
+    - apply TViewFacts.write_fence_sc_incr.
+  Qed.
+
+  Lemma program_step_future
+        e lc1 gl1 lc2 gl2
+        (STEP: program_step e lc1 gl1 lc2 gl2)
+        (LC_WF1: wf lc1 gl1)
+        (GL_WF1: Global.wf gl1):
+    <<LC_WF2: wf lc2 gl2>> /\
+    <<GL_WF2: Global.wf gl2>> /\
+    <<TVIEW_FUTURE: TView.le (tview lc1) (tview lc2)>> /\
+    <<SC_FUTURE: TimeMap.le (Global.sc gl1) (Global.sc gl2)>> /\
+    <<MEM_FUTURE: Memory.future (Global.memory gl1) (Global.memory gl2)>>.
+  Proof.
+    inv STEP; try by (esplits; eauto; try refl).
+    - exploit read_step_future; eauto. i. des.
+      esplits; eauto; try refl.
+    - exploit write_step_future; eauto;
+        (try by econs); try apply Time.bot_spec. i. des.
+      esplits; eauto; try refl.
+    - exploit read_step_future; eauto. i. des.
+      exploit write_step_future; eauto; try by econs.
+      { etrans; eauto. inv LOCAL2.
+        econs. eauto using Memory.add_ts.
+      }
+      i. des.
+      esplits; eauto. etrans; eauto.
+    - exploit fence_step_future; eauto.
+    - exploit fence_step_future; eauto.
+  Qed.
+
+  Lemma internal_step_inhabited
+        e lc1 gl1 lc2 gl2
+        (STEP: internal_step e lc1 gl1 lc2 gl2)
+        (INHABITED1: Memory.inhabited (Global.memory gl1)):
+    <<INHABITED2: Memory.inhabited (Global.memory gl2)>>.
+  Proof.
+    inv STEP; inv LOCAL; ss.
+  Qed.
+
+  Lemma program_step_inhabited
+        e lc1 gl1 lc2 gl2
+        (STEP: program_step e lc1 gl1 lc2 gl2)
+        (INHABITED1: Memory.inhabited (Global.memory gl1)):
+    <<INHABITED2: Memory.inhabited (Global.memory gl2)>>.
+  Proof.
+    inv STEP; eauto.
+    - inv LOCAL. eauto using Memory.add_inhabited.
+    - inv LOCAL2. eauto using Memory.add_inhabited.
+    - inv LOCAL. ss.
+    - inv LOCAL. ss.
+  Qed.
+
+
+  (* step_disjoint *)
+
+  Lemma promise_step_disjoint
+        lc1 sc1 mem1 loc from to msg lc2 mem2 lc kind
+        (STEP: promise_step lc1 gl1 loc lc2 mem2 kind)
+        (WF1: wf lc1 mem1)
+        (SC1: Memory.closed_timemap sc1 mem1)
+        (CLOSED1: Memory.closed mem1)
+        (DISJOINT1: disjoint lc1 lc)
+        (WF: wf lc mem1):
+    <<DISJOINT2: disjoint lc2 lc>> /\
+    <<WF: wf lc mem2>>.
+  Proof.
+    inv WF1. inv DISJOINT1. inversion WF. inv STEP.
+    exploit Memory.promise_future; try apply PROMISE; eauto. i. des.
+    exploit Memory.promise_disjoint; try apply PROMISE; eauto. i. des.
+    splits; ss. econs; eauto.
+    eapply TView.future_closed; eauto.
+  Qed.
+
+  Lemma read_step_disjoint
+        lc1 mem1 lc2 loc ts val released ord lc
+        (STEP: read_step lc1 mem1 loc ts val released ord lc2)
+        (WF1: wf lc1 mem1)
+        (DISJOINT1: disjoint lc1 lc)
+        (WF: wf lc mem1):
+    disjoint lc2 lc.
+  Proof.
+    inv WF1. inv DISJOINT1. inv WF. inv STEP. ss.
+  Qed.
+
+  Lemma write_step_disjoint
+        lc1 sc1 mem1 lc2 sc2 loc from to val releasedm released ord mem2 kind lc
+        (STEP: write_step lc1 sc1 mem1 loc from to val releasedm released ord lc2 sc2 mem2 kind)
+        (WF1: wf lc1 mem1)
+        (SC1: Memory.closed_timemap sc1 mem1)
+        (CLOSED1: Memory.closed mem1)
+        (DISJOINT1: disjoint lc1 lc)
+        (WF: wf lc mem1):
+    <<DISJOINT2: disjoint lc2 lc>> /\
+    <<WF: wf lc mem2>>.
+  Proof.
+    inv WF1. inv DISJOINT1. inversion WF. inv STEP.
+    exploit Memory.write_disjoint; try apply WRITE; eauto. i. des.
+    splits; ss. econs; eauto.
+    inv WRITE. eapply TView.promise_closed; eauto.
+  Qed.
+
+  Lemma write_na_step_disjoint
+        lc1 sc1 mem1 loc from to val ord lc2 sc2 mem2 msgs kinds kind lc
+        (STEP: write_na_step lc1 sc1 mem1 loc from to val ord lc2 sc2 mem2 msgs kinds kind)
+        (WF1: wf lc1 mem1)
+        (SC1: Memory.closed_timemap sc1 mem1)
+        (CLOSED1: Memory.closed mem1)
+        (DISJOINT1: disjoint lc1 lc)
+        (WF: wf lc mem1):
+    <<DISJOINT2: disjoint lc2 lc>> /\
+    <<WF: wf lc mem2>>.
+  Proof.
+    exploit write_na_step_future; eauto. i. des.
+    inv WF1. inv DISJOINT1. inversion WF. inv STEP.
+    exploit Memory.write_na_disjoint; try apply WRITE; eauto. i. des.
+    splits; ss. econs; eauto.
+    eapply TView.future_closed; eauto.
+  Qed.
+
+  Lemma fence_step_disjoint
+        lc1 sc1 mem1 lc2 sc2 ordr ordw lc
+        (STEP: fence_step lc1 sc1 ordr ordw lc2 sc2)
+        (WF1: wf lc1 mem1)
+        (SC1: Memory.closed_timemap sc1 mem1)
+        (DISJOINT1: disjoint lc1 lc)
+        (WF: wf lc mem1):
+    <<DISJOINT2: disjoint lc2 lc>> /\
+    <<WF: wf lc mem1>>.
+  Proof.
+    inv WF1. inv DISJOINT1. inv WF. inv STEP. splits; ss.
+  Qed.
+
+  Lemma read_step_promises
+        lc1 mem loc to val released ord lc2
+        (READ: read_step lc1 mem loc to val released ord lc2):
+    (promises lc1) = (promises lc2).
+  Proof.
+    inv READ. auto.
+  Qed.
+
+  Lemma program_step_disjoint
+        e lc1 sc1 mem1 lc2 sc2 mem2 lc
+        (STEP: program_step e lc1 sc1 mem1 lc2 sc2 mem2)
+        (WF1: wf lc1 mem1)
+        (SC1: Memory.closed_timemap sc1 mem1)
+        (CLOSED1: Memory.closed mem1)
+        (DISJOINT1: disjoint lc1 lc)
+        (WF: wf lc mem1):
+    <<DISJOINT2: disjoint lc2 lc>> /\
+    <<WF: wf lc mem2>>.
+  Proof.
+    inv STEP; try by (esplits; eauto).
+    - exploit read_step_disjoint; eauto.
+    - exploit write_step_disjoint; eauto.
+    - exploit read_step_future; eauto. i. des.
+      exploit read_step_disjoint; eauto. i. des.
+      exploit write_step_disjoint; eauto.
+    - exploit fence_step_disjoint; eauto.
+    - exploit fence_step_disjoint; eauto.
+    - exploit write_na_step_disjoint; eauto.
+  Qed.
+
+  Lemma program_step_promises_bot
+        e lc1 sc1 mem1 lc2 sc2 mem2
+        (STEP: program_step e lc1 sc1 mem1 lc2 sc2 mem2)
+        (PROMISES: (promises lc1) = Memory.bot):
+    (promises lc2) = Memory.bot.
+  Proof.
+    inv STEP; try inv LOCAL; ss.
+    - eapply Memory.write_promises_bot; eauto.
+    - inv LOCAL1. inv LOCAL2.
+      eapply Memory.write_promises_bot; eauto.
+    - eapply Memory.write_na_promises_bot; eauto.
+  Qed.
+
+  Lemma program_step_get_diff_promises
+        l
+        e lc1 sc1 mem1 lc2 sc2 mem2
+        (STEP: program_step e lc1 sc1 mem1 lc2 sc2 mem2)
+        (LOC: ~ ThreadEvent.is_accessing_loc l e):
+    forall to, Memory.get l to lc1.(promises) = Memory.get l to lc2.(promises).
+  Proof.
+    inv STEP; ss; try by inv LOCAL.
+    - i. inv LOCAL. s.
+      erewrite <- Memory.write_get_diff_promise; eauto.
+    - i. inv LOCAL1. inv LOCAL2. s.
+      erewrite <- Memory.write_get_diff_promise; eauto.
+    - i. inv LOCAL.
+      erewrite <- Memory.write_na_get_diff_promise; eauto.
+  Qed.
+
+  Lemma program_step_get_diff
+        l
+        e lc1 sc1 mem1 lc2 sc2 mem2
+        (STEP: program_step e lc1 sc1 mem1 lc2 sc2 mem2)
+        (LOC: ~ ThreadEvent.is_accessing_loc l e):
+    forall to, Memory.get l to mem1 = Memory.get l to mem2.
+  Proof.
+    inv STEP; ss; try by inv LOCAL.
+    - i. inv LOCAL. s.
+      erewrite <- Memory.write_get_diff; eauto.
+    - i. inv LOCAL1. inv LOCAL2. s.
+      erewrite <- Memory.write_get_diff; eauto.
+    - i. inv LOCAL.
+      erewrite <- Memory.write_na_get_diff; try exact WRITE; eauto.
+  Qed.
+
+  Lemma promise_step_non_promised
+        lc1 mem1 loc from to msg lc2 mem2 kind
+        l f t m
+        (STEP: promise_step lc1 mem1 loc from to msg lc2 mem2 kind)
+        (GET: Memory.get l t mem1 = Some (f, m))
+        (GETP: Memory.get l t lc1.(Local.promises) = None):
+    (<<GET: Memory.get l t mem2 = Some (f, m)>>) /\
+    (<<GETP: Memory.get l t lc2.(Local.promises) = None>>).
+  Proof.
+    inv STEP. eauto using Memory.promise_non_promised.
+  Qed.
+
+  Lemma program_step_non_promised
+        e lc1 sc1 mem1 lc2 sc2 mem2
+        l f t m
+        (STEP: program_step e lc1 sc1 mem1 lc2 sc2 mem2)
+        (GET: Memory.get l t mem1 = Some (f, m))
+        (GETP: Memory.get l t lc1.(Local.promises) = None):
+    (<<GET: Memory.get l t mem2 = Some (f, m)>>) /\
+    (<<GETP: Memory.get l t lc2.(Local.promises) = None>>).
+  Proof.
+    inv STEP; eauto; try by (inv LOCAL; eauto).
+    - inv LOCAL.
+      eauto using Memory.write_non_promised.
+    - inv LOCAL1. inv LOCAL2.
+      eauto using Memory.write_non_promised.
+    - inv LOCAL.
+      eauto using Memory.write_na_non_promised.
+  Qed.
+End Local.
